proof/LinearContext.v
@@ -1,23 +1,15 @@
 Set Warnings "-notation-overridden,-parsing".
 From PLF Require Import Maps.
+From PLF Require Import Ax.
 From Coq Require Import Lists.List.
 Import ListNotations.
+Import Ax.
 
 Definition linear_context (A : Type) := list (string * A).
 
 Definition l_empty {A:Type} : linear_context A := nil.
 
 (* Implemenetd as find the right most one *)
-
-Fixpoint l_find_right_most {A:Type} (ctx: linear_context A) (name: string) :=
-  match ctx with
-  | [] => None
-  | (x, xty)::ctx =>
-      match l_find_right_most ctx name with
-      | None => if String.eqb x name then Some xty else None
-      | Some xty => Some xty
-      end
-  end.
 
 Definition l_append {A : Type} (m : linear_context A) (x : string) (v : A) : linear_context A := m ++ [(x, v)].
 
@@ -47,6 +39,18 @@ Proof. intros. apply app_eq_unit in H.
 Qed.
 
 Global Hint Resolve app_list_unit_eq_unit: core.
+
+
+Fixpoint l_find_right_most {A:Type} (ctx: list (prod string A)) (name: string) :=
+  match ctx with
+  | nil => None
+  | (x, xty)::ctx =>
+      match l_find_right_most ctx name with
+      | None => if String.eqb x name then Some xty else None
+      | Some xty => Some xty
+      end
+  end.
+
 
 Lemma l_find_right_most_none_neq_hd {A: Type}: forall (Gamma: linear_context A) x tx a,
     l_find_right_most ((x, tx):: Gamma) a = None -> x <> a.
@@ -116,13 +120,93 @@ Proof with eauto.
       simpl in H. rewrite HH in H. destruct (eqb_spec s name); subst... exfalso... inversion H1.
 Qed.
 
-Lemma l_find_right_most_some_spec {A:Type}: forall (ctx: linear_context A) (name: string) (tau: A),
+Lemma l_find_right_most_some_spec_aux {A:Type}: forall (ctx: list (prod string A)) (name: string) (tau: A),
+  l_find_right_most ctx name = Some tau ->
+  (exists ctx1 ctx2,
+      ctx = ctx1 ++ ((name, tau)::nil) ++ ctx2
+  ).
+Proof with auto.
+  intros.
+  apply l_find_implies_in in H. apply in_split in H. destruct H as (G1 & G2 & HG12).
+  exists G1, G2. subst. split...
+Qed.
+
+Lemma l_find_right_most_last_eq {A:Type}: forall (ctx: list (prod string A)) name tau,
+    l_find_right_most (ctx ++ [(name, tau)]) name = Some tau.
+Proof with eauto.
+  intros. induction ctx...
+  - simpl. rewrite eqb_refl...
+  - destruct a.
+    destruct (eqb_spec s name); subst...
+    simpl. rewrite IHctx...
+    simpl. rewrite IHctx...
+Qed.
+
+Lemma l_find_right_most_last_neq_none {A:Type}: forall (ctx: list (prod string A)) name tau a,
+    name <> a ->
+    l_find_right_most (ctx ++ [(name, tau)]) a = None <->
+      l_find_right_most ctx a = None.
+Proof with eauto.
+  intros. induction ctx...
+  - simpl. split; intros...
+    destruct (eqb_spec name a); subst... exfalso...
+  - split; intros.
+    + destruct a0. simpl in H0.
+      destruct (l_find_right_most (ctx ++ [(name, tau)]) a) eqn : HH... inversion H0.
+      destruct (eqb_spec s a); subst... inversion H0. simpl.
+      destruct (l_find_right_most ctx a)... rewrite IHctx in H0. inversion H0.
+      destruct (eqb_spec s a); subst... exfalso...
+    + destruct a0. simpl in H0. simpl.
+      destruct (l_find_right_most ctx a) eqn : HH... inversion H0.
+      destruct (l_find_right_most (ctx ++ [(name, tau)])) eqn: HHH...
+      assert (Some a1 = None)... rewrite IHctx...
+Qed.
+
+Lemma l_find_right_most_last_neq {A:Type}: forall (ctx: list (prod string A)) name tau a tau_a,
+    name <> a ->
+    l_find_right_most (ctx ++ [(name, tau)]) a = Some tau_a <->
+      l_find_right_most ctx a = Some tau_a.
+Proof with eauto.
+  intros. induction ctx...
+  - simpl. split; intros.
+    destruct (eqb_spec name a); subst... exfalso... inversion H0.
+  - split; intros.
+    + destruct a0. simpl in H0.
+      destruct (l_find_right_most (ctx ++ [(name, tau)]) a) eqn : HH...
+      simpl. rewrite IHctx in H0. rewrite H0...
+      destruct (eqb_spec s a); subst... inversion H0; subst... apply l_find_right_most_weak_pre in HH.
+      simpl. rewrite HH. rewrite eqb_refl... inversion H0.
+    + destruct a0. simpl in H0. simpl.
+      destruct (l_find_right_most ctx a) eqn : HH...
+      simpl. rewrite <- IHctx in H0. rewrite H0...
+      assert (l_find_right_most (ctx ++ [(name, tau)]) a = None). rewrite l_find_right_most_last_neq_none...
+      rewrite H1.
+      destruct (eqb_spec s a); subst...
+Qed.
+
+Lemma l_find_right_most_some_spec {A:Type}: forall (ctx: list (prod string A)) (name: string) (tau: A),
   l_find_right_most ctx name = Some tau ->
   (exists ctx1 ctx2,
       ctx = ctx1 ++ ((name, tau)::nil) ++ ctx2 /\ l_find_right_most ctx2 name = None
   ).
 Proof with auto.
-Admitted.
+  apply (rev_ind (fun ctx => forall name tau,
+                      l_find_right_most ctx name = Some tau ->
+                      (exists ctx1 ctx2,
+                          ctx = ctx1 ++ ((name, tau)::nil) ++ ctx2 /\ l_find_right_most ctx2 name = None
+                      )
+        )).
+  - intros name tau Hfind. inversion Hfind.
+  - intros (a, tau_a) ctx Hind name tau Hfind.
+    destruct (eqb_spec a name); subst.
+    + exists ctx, nil. split... rewrite app_nil_r. rewrite l_find_right_most_last_eq in Hfind. inversion Hfind; subst...
+    + assert (l_find_right_most ctx name = Some tau). erewrite l_find_right_most_last_neq in Hfind...
+      apply Hind in H. destruct H as (ctx1 & ctx2 & Hctx12 & Hfind12).
+      exists ctx1, (ctx2 ++ ((a, tau_a)::nil)).
+      split... rewrite Hctx12. rewrite <- app_assoc. rewrite <- app_assoc...
+      rewrite l_find_right_most_last_neq_none...
+Qed.
+
 (*   intros. *)
 (*   apply l_find_implies_in in H. apply in_split in H. destruct H as (G1 & G2 & HG12). *)
 (*   exists G1, G2. subst. split... *)
