proof/Ax.v
@@ -1,12 +1,14 @@
 Set Warnings "-notation-overridden,-parsing".
 From PLF Require Import Maps.
-From PLF Require Import Types.
+(* From PLF Require Import Types. *)
 (* From PLF Require Import Smallstep. *)
 From PLF Require Import CoreLangSimp.
 From PLF Require Import NormalTypeSystemSimp.
 From Coq Require Import Logic.FunctionalExtensionality.
 From Coq Require Import Logic.ClassicalFacts.
 
+From Coq Require Import Lists.List.
+Import ListNotations.
 Import NormalTypeSystemSimp.
 
 Definition state_permute {A:Type}: forall (st: string -> option A) x y (a a': A),
@@ -19,9 +21,30 @@ Admitted.
 Lemma closed_term_has_no_free_var: forall e x T, empty \N- e \Tin T -> ~ x \FVtm e.
 Admitted.
 
-(* for vfix Axiom *)
-Definition const_order: constant -> constant -> Prop.
+Lemma lete_preserve_not_free: forall e x a e_a, ~ x \FVtm e_a -> ~ x \FVtm e -> ~ x \FVtm tlete a e_a e.
+Proof with eauto.
 Admitted.
 
+Global Hint Resolve lete_preserve_not_free: core.
+
+Definition const_order (c1 c2: constant) : Prop :=
+  match c1 with
+  | cbool c1 =>
+      match c2 with
+      | cbool c2 =>
+          (match c1 with
+           | true => False
+           | false => c2 = true
+           end)
+      | cnat _ => True
+      end
+  | cnat c1 =>
+      match c2 with
+      | cbool _ => False
+      | cnat c2 => c1 < c2
+      end
+  end.
+
+(* for vfix Axiom *)
 Lemma const_order_is_well_founded: well_founded const_order.
 Admitted.
