proof/TermMeet.v
@@ -19,61 +19,93 @@ Import CoreLangSimp.
 Import NormalTypeSystemSimp.
 Import LinearContext.
 Import NoDup.
+Import Ax.
 Import RfTypeDef.
 Import TypeClosedSimp.
 Import DenotationSimp.
 Import WellFormedSimp.
 Import ListNotations.
 
-(* meet operation, the trick here is encode the conjunction into the target language, via a poly equal operator.
-
-  let x1 = e1 in
-  let x2 = e2 in
-  let x3 = x1 ==T x2 in
-  match x3 with
-  | true -> x2
-  | false -> err
-
- *)
-Lemma meet_of_two_terms_exists: forall e1 e2 T,
-    empty \N- e1 \Tin T -> empty \N- e2 \Tin T -> (exists e3, (empty \N- e3 \Tin T) /\ (forall c, e3 -->* c <-> e1 -->* c /\ e2 -->* c)).
-Admitted.
-
-Lemma meet_of_two_terms_implies_denotation: forall st tau e1 e2 e3,
-    tmR_aux st tau e1 -> tmR_aux st tau e2 ->
-    (forall c, e3 -->* c <-> e1 -->* c /\ e2 -->* c) -> tmR_aux st tau e3.
-Admitted.
-
-Lemma meet_of_two_terms_term_order: forall e1 e2 e3,
+Lemma meet_of_two_terms_term_order: forall e1 e2 e3 T,
+    empty \N- e1 \Tin T -> empty \N- e2 \Tin T -> empty \N- e3 \Tin T ->
     (forall c, e3 -->* c <-> e1 -->* c /\ e2 -->* c) -> (e3 <-< e1) /\ (e3 <-< e2).
-Admitted.
+Proof with eauto.
+  intros.
+  split.
+  - split... intros. rewrite H2 in H3... destruct H3...
+    intros. apply weakening_empty with (Gamma := Gamma) in H1.
+    assert (T0 = T). eapply ty_unique... subst... eapply  weakening_empty...
+  - split... intros. rewrite H2 in H3... destruct H3...
+    intros. apply weakening_empty with (Gamma := Gamma) in H1.
+    assert (T0 = T). eapply ty_unique... subst... eapply  weakening_empty...
+Qed.
 
 Lemma meet_of_three_terms_exists: forall e1 e2 e3 T,
     empty \N- e1 \Tin T -> empty \N- e2 \Tin T -> empty \N- e3 \Tin T ->
     (exists e, (empty \N- e \Tin T) /\
             (forall c, e -->* c <-> e1 -->* c /\ e2 -->* c /\ e3 -->* c)).
-Admitted.
+Proof with eauto.
+  intros.
+  destruct (meet_of_two_terms_exists e1 e2 T) as (e4 & HTe4 & HEe4)...
+  destruct (meet_of_two_terms_exists e4 e3 T) as (e5 & HTe5 & HEe5)...
+  exists e5. split...
+  intro c. split... intros... apply HEe5 in H2. destruct H2. apply HEe4 in H2. destruct H2...
+  intros. rewrite HEe5. destruct H2 as (H21 & H22 & H23)... split... apply HEe4...
+Qed.
 
-Lemma meet_of_three_terms_implies_denotation: forall st tau e1 e2 e3 e,
-    tmR_aux st tau e1 -> tmR_aux st tau e2 -> tmR_aux st tau e3 ->
-    (forall c, e -->* c <-> e1 -->* c /\ e2 -->* c /\ e3 -->* c) -> tmR_aux st tau e.
-Admitted.
-
-Lemma meet_of_three_terms_term_order: forall e1 e2 e3 e,
+Lemma meet_of_three_terms_term_order: forall e1 e2 e3 e T,
+    empty \N- e1 \Tin T -> empty \N- e2 \Tin T -> empty \N- e3 \Tin T -> empty \N- e \Tin T ->
     (forall c, e -->* c <-> e1 -->* c /\ e2 -->* c /\ e3 -->* c) -> (e <-< e1) /\ (e <-< e2) /\ (e <-< e3).
-Admitted.
+Proof with eauto.
+  intros.
+  split.
+  - split... intros. rewrite H3 in H4... destruct H4...
+    intros. apply weakening_empty with (Gamma := Gamma) in H2.
+    assert (T0 = T). eapply ty_unique... subst... eapply  weakening_empty...
+  - split...
+    split...
+    intros. rewrite H3 in H4... destruct H4... destruct H5...
+    intros. assert (Gamma \N- e \Tin T). eapply weakening_empty in H2...
+    assert (T = T0). eapply ty_unique... subst... eapply  weakening_empty...
+    split...
+    intros. rewrite H3 in H4... destruct H4... destruct H5...
+    intros. assert (Gamma \N- e \Tin T). eapply weakening_empty in H2...
+    assert (T = T0). eapply ty_unique... subst... eapply  weakening_empty...
+Qed.
+
 
 Lemma meet_of_four_terms_exists: forall e1 e2 e3 e4 T,
     empty \N- e1 \Tin T -> empty \N- e2 \Tin T -> empty \N- e3 \Tin T -> empty \N- e4 \Tin T ->
     (exists e, (empty \N- e \Tin T) /\
             (forall c, e -->* c <-> e1 -->* c /\ e2 -->* c /\ e3 -->* c /\ e4 -->* c)).
-Admitted.
+Proof with eauto.
+  intros.
+  destruct (meet_of_three_terms_exists e1 e2 e3 T) as (e123 & HTe123 & HEe123)...
+  destruct (meet_of_two_terms_exists e123 e4 T) as (e & HTe & HEe)...
+  exists e. split...
+  intro c. split... intros... apply HEe in H3. destruct H3. apply HEe123 in H3... destruct H3 as (Ha & Hb & Hc)...
+  intros. rewrite HEe. destruct H3 as (H21 & H22 & H23 & H4)... split... apply HEe123...
+Qed.
 
-Lemma meet_of_four_terms_implies_denotation: forall st tau e1 e2 e3 e4 e,
-    tmR_aux st tau e1 -> tmR_aux st tau e2 -> tmR_aux st tau e3 ->
-    (forall c, e -->* c <-> e1 -->* c /\ e2 -->* c /\ e3 -->* c /\ e4 -->* c) -> tmR_aux st tau e.
-Admitted.
-
-Lemma meet_of_four_terms_term_order: forall e1 e2 e3 e4 e,
+Lemma meet_of_four_terms_term_order: forall e1 e2 e3 e4 e T,
+    empty \N- e1 \Tin T -> empty \N- e2 \Tin T -> empty \N- e3 \Tin T -> empty \N- e4 \Tin T -> empty \N- e \Tin T ->
     (forall c, e -->* c <-> e1 -->* c /\ e2 -->* c /\ e3 -->* c /\ e4 -->* c) -> (e <-< e1) /\ (e <-< e2) /\ (e <-< e3) /\ (e <-< e4).
-Admitted.
+Proof with eauto.
+  intros.
+  split.
+  - split... intros. rewrite H4 in H5... destruct H5...
+    intros. apply weakening_empty with (Gamma := Gamma) in H3.
+    assert (T0 = T). eapply ty_unique... subst... eapply  weakening_empty...
+  - split...
+    split...
+    intros. rewrite H4 in H5... destruct H5... destruct H6...
+    intros. apply weakening_empty with (Gamma := Gamma) in H3.
+    assert (T0 = T). eapply ty_unique... subst... eapply  weakening_empty...
+    split...
+    split. intros. rewrite H4 in H5... destruct H5... destruct H6... destruct H7...
+    intros. apply weakening_empty with (Gamma := Gamma) in H3.
+    assert (T0 = T). eapply ty_unique... subst... eapply  weakening_empty...
+    split. intros. rewrite H4 in H5... destruct H5... destruct H6... destruct H7...
+    intros. apply weakening_empty with (Gamma := Gamma) in H3.
+    assert (T0 = T). eapply ty_unique... subst... eapply  weakening_empty...
+Qed.
